lifter: implement expression lifting of ror and rol
Notice that this general lifting has not been instantiated for the M0
and ARM8 lifters, yet

src/tools/lifter/bir_inst_liftingLib.sml
@@ -871,7 +871,8 @@ functor bir_inst_liftingFunctor (MD : sig val mr : bmr_rec end) : bir_inst_lifti
          bir_nzcv_expTheory.BExp_nzcv_ADD_vars_of, bir_nzcv_expTheory.BExp_nzcv_SUB_vars_of,
          bir_nzcv_expTheory.BExp_ADD_WITH_CARRY_vars_of,
          BExp_word_reverse_vars_of, BExp_Align_vars_of, BExp_Aligned_vars_of,
-         BExp_MSB_vars_of, BExp_LSB_vars_of, BExp_word_bit_vars_of, BExp_word_bit_exp_vars_of]
+         BExp_MSB_vars_of, BExp_LSB_vars_of, BExp_word_bit_vars_of, BExp_word_bit_exp_vars_of,
+         BExp_ror_vars_of, BExp_ror_exp_vars_of, BExp_rol_vars_of, BExp_rol_exp_vars_of]
 
      val comp_upd_imm_varname_conv = SIMP_CONV (list_ss++stringSimps.STRING_ss) [bir_temp_varsTheory.bir_temp_var_def, bir_envTheory.bir_var_name_def, bir_temp_varsTheory.bir_temp_var_name_def]
 
